prove ttl example

src/Examples/Ttl/Ttl.v
@@ -35,7 +35,7 @@ Module Ttl.
   (*   hlist.t ["field1"; …; "ttl"] [Semantics.byte; …; Semantics.byte]. (* field1, ttl *) *)
 
   Definition packet :=
-    Vector.t Semantics.byte 2. (* field1, ttl *)
+    Vector.t Semantics.word 2. (* field1, ttl *)
 
   Local Declare Scope sep_scope.
   Local Delimit Scope sep_scope with sep.
@@ -48,15 +48,16 @@ Module Ttl.
   Notation field1 p := (Vector.nth p field1_index).
   Notation ttl p := (Vector.nth p ttl_index).
 
-  Definition ByteVector {n} (addr: address) (v: Vector.t Semantics.byte n) : Semantics.mem -> Prop :=
-    array ptsto (word.of_Z 1) addr (Vector.to_list v).
+  Definition WordVector {n} (addr: address) (v: Vector.t Semantics.word n) : Semantics.mem -> Prop :=
+    array scalar (word.of_Z 8) addr (Vector.to_list v).
 
   Definition Packet (addr: address) (p: packet) : Semantics.mem -> Prop :=
-    ByteVector addr p.
+    WordVector addr p.
 
   Definition decr_gallina (p: packet) :=
     let/d ttl := (ttl p) in
-    let/d ttl := word.sub ttl (word.of_Z 1) in
+    let/d m1 := word.of_Z (-1) in
+    let/d ttl := word.add ttl m1 in
     let/d p := Vector.replace p ttl_index ttl in
     p.
 
@@ -75,31 +76,89 @@ Module Ttl.
     Datatypes.length (Vector.to_list v) = n.
   Proof. Admitted.
 
+  Lemma compile_nth :
+    forall (locals: Semantics.locals) (mem: Semantics.mem)
+      tr R R' functions T (pred: T -> _ -> Prop)
+      {n} (vector: Vector.t Semantics.word n) vector_ptr vector_var
+      offset var k k_impl,
+      (Z.of_nat n < 2 ^ Semantics.width)%Z ->
+      sep (WordVector vector_ptr vector) R' mem ->
+      map.get locals vector_var = Some vector_ptr ->
+      let v := Vector.nth vector offset in
+      let noffset := proj1_sig (Fin.to_nat offset) in
+      (let head := v in
+       forall m,
+         sep (WordVector vector_ptr vector) R' m ->
+         (find k_impl
+          implementing (pred (k head))
+          with-locals (map.put locals var head)
+          and-memory m and-trace tr and-rest R
+          and-functions functions)) ->
+      (let head := v in
+       find (cmd.seq (cmd.set
+                        var
+                        (expr.load
+                           access_size.word
+                           (expr.op bopname.add
+                                    (expr.var vector_var)
+                                    (expr.literal ((word.unsigned (word.of_Z 8) * Z.of_nat noffset))))))
+                     k_impl)
+       implementing (pred (dlet head k))
+       with-locals locals and-memory mem and-trace tr and-rest R
+       and-functions functions).
+  Proof.
+    intros.
+    unfold WordVector in *.
+    repeat straightline.
+    exists (word.of_Z (word.unsigned v)).
+    split.
+    { repeat straightline; eauto.
+      exists vector_ptr; intuition.
+      seprewrite_in @array_index_nat_inbounds H0;
+        cycle 1.
+      { eexists.
+        split.
+        { eapply load_word_of_sep.
+          ecancel_assumption. }
+      { subst v.
+        (* FIXME: vector/list lemmas *)
+        admit. } }
+      { rewrite Vector_to_list_length.
+        apply (proj2_sig (Fin.to_nat offset)). } }
+    { repeat straightline.
+      cbv [dlet.dlet].
+      subst l.
+      rewrite word.of_Z_unsigned.
+      eauto. }
+    Unshelve.
+    apply (word.of_Z 0).
+    Admitted.
+
   Lemma compile_replace :
     forall (locals: Semantics.locals) (mem: Semantics.mem)
       tr R R' functions T (pred: T -> _ -> Prop)
-      {n} (vector: Vector.t Semantics.byte n) vector_ptr vector_var
+      {n} (vector: Vector.t Semantics.word n) vector_ptr vector_var
       value value_var offset
       k k_impl,
       (Z.of_nat n < 2 ^ Semantics.width)%Z ->
-      sep (ByteVector vector_ptr vector) R' mem ->
+      sep (WordVector vector_ptr vector) R' mem ->
       map.get locals vector_var = Some vector_ptr ->
       map.get locals value_var = Some value ->
-      let v := (Vector.replace vector offset (word.of_Z (word.unsigned value))) in
-      let zoffset := Z.of_nat (proj1_sig (Fin.to_nat offset)) in
+      let v := (Vector.replace vector offset value) in
+      let noffset := proj1_sig (Fin.to_nat offset) in
       (let head := v in
        forall m,
-         sep (ByteVector vector_ptr head) R' m ->
+         sep (WordVector vector_ptr head) R' m ->
          (find k_impl
           implementing (pred (k head))
           with-locals locals
           and-memory m and-trace tr and-rest R
           and-functions functions)) ->
       (let head := v in
-       find (cmd.seq (cmd.store access_size.one
+       find (cmd.seq (cmd.store access_size.word
                                 (expr.op bopname.add
                                          (expr.var vector_var)
-                                         (expr.literal zoffset))
+                                         (expr.literal ((word.unsigned (word.of_Z 8) * Z.of_nat noffset))))
                                 (expr.var value_var))
                      k_impl)
        implementing (pred (dlet head k))
@@ -107,9 +166,10 @@ Module Ttl.
        and-functions functions).
   Proof.
     intros.
-    unfold ByteVector in *.
+    unfold WordVector in *.
     repeat straightline.
-    exists (word.add vector_ptr (word.of_Z zoffset)).
+    exists (word.add vector_ptr
+                     (word.of_Z (word.unsigned (word.of_Z 8) * Z.of_nat noffset))).
     split.
     { repeat straightline; eauto.
       exists vector_ptr; intuition.
@@ -119,60 +179,25 @@ Module Ttl.
       { straightline.
         eexists; eauto. }
       { repeat straightline.
-        eapply store_one_of_sep.
-        { pose proof (vector_uncons vector).
-          (let lemma0 := open_constr:(bytearray_index_inbounds
-                                       (Vector.to_list vector)
-                                       vector_ptr
-                                       (word.of_Z zoffset) _) in
-           let t := type of lemma0 in
-           let t := (eval cbv zeta in t) in
-           let lemma1 := open_constr:(lemma0 : t) in
-           seprewrite0_in lemma1 H0).
-          ecancel_assumption.
-          Unshelve.
-          subst zoffset.
-          rewrite word.unsigned_of_Z.
-          pose proof (proj2_sig (Fin.to_nat offset)) as Hlt.
-          simpl in Hlt.
-          rewrite Vector_to_list_length.
-          unfold word.wrap.     (* FIXME lemmify *)
-          rewrite Z.mod_small.
-          { apply Nat2Z.inj_lt; eauto. }
-          { split.
-            { apply Zle_0_nat. }
-            { etransitivity.
-              { apply Nat2Z.inj_lt.
-                eassumption. }
-              { eassumption. } } } }
+        eapply store_word_of_sep.
+        { seprewrite_in @array_index_nat_inbounds H0;
+            cycle 1.
+          { ecancel_assumption. }
+          { subst noffset.
+            rewrite Vector_to_list_length.
+            apply (proj2_sig (Fin.to_nat offset)). } }
         { intros.
           apply H3.
-          (let lemma0 := open_constr:(bytearray_index_inbounds
-                                       (Vector.to_list v)
-                                       vector_ptr
-                                       (word.of_Z zoffset) _) in
-           let t := type of lemma0 in
-           let t := (eval cbv zeta in t) in
-           let lemma1 := open_constr:(lemma0 : t) in
-           seprewrite0 lemma1).
-          admit.                (* Lemmas on Vector.to_list and replace *)
-          Unshelve.
-          subst zoffset.
-          rewrite word.unsigned_of_Z.
-          pose proof (proj2_sig (Fin.to_nat offset)) as Hlt.
-          simpl in Hlt.
-          rewrite Vector_to_list_length.
-          unfold word.wrap.     (* FIXME lemmify *)
-          rewrite Z.mod_small.
-          { apply Nat2Z.inj_lt; eauto. }
-          { split.
-            { apply Zle_0_nat. }
-            { etransitivity.
-              { apply Nat2Z.inj_lt.
-                eassumption. }
-              { eassumption. } } } }
+          seprewrite (array_index_nat_inbounds (default:=word.of_Z 0) scalar (word.of_Z 8) (Vector.to_list v) vector_ptr (proj1_sig (Fin.to_nat offset))); cycle 1.
+          { admit.                (* Lemmas on Vector.to_list and replace *)
+          }
+          { subst noffset.
+            rewrite Vector_to_list_length.
+            apply (proj2_sig (Fin.to_nat offset)). } }
   Admitted.
 
+  Hint Unfold Packet : compiler.
+  Opaque dlet.
 
   Derive decr_body SuchThat
        (let decr := ("decr", (["p"], [], decr_body)) in
@@ -189,4 +214,15 @@ Module Ttl.
     As decr_body_correct.
   Proof.
     setup.
+    assert (Z.of_nat 2 < 2 ^ Semantics.width)%Z by (cbn; lia).
+    eapply compile_nth with (var := "ttl").
+    1-3:repeat t; eauto.
+    do 6 t.
+    1-2:repeat t.
+    intros.
+    eapply compile_replace.
+    1-4:repeat t; eauto.
     repeat t.
+  Qed.
+End Ttl.
+
